case_study/RiscvPmp/BlockVer/Examples.v
@@ -35,6 +35,7 @@ From Katamaran Require Import
      Notations
      Bitvector
      Semantics
+     Instance
      RiscvPmp.BlockVer.Spec
      RiscvPmp.BlockVer.PartialVerifier
      RiscvPmp.Machine
@@ -272,7 +273,7 @@ Module Examples.
       Import RiscvPmpBlockVerifIrisInstance.
       Import RiscvPmpIrisInstanceWithContracts.
 
-      Context `{sailGS Σ} {rG : iostateG IOState Σ}.
+      Context `{sailGS Σ} {rG : trivGS Σ}.
 
       Definition ptsto_instrs_from_contract {Γ} (c : @BlockVerifierContract Γ) (a : Val ty_xlenbits) : iProp Σ :=
         ptsto_instrs a (extract_instrs_from_contract c).
